theories/lang/bi/atomic1.v
@@ -1,0 +1,610 @@
+(*
+ * Copyright (C) BedRock Systems Inc. 2020
+ *
+ * SPDX-License-Identifier: LGPL-2.1 WITH BedRock Exception for use over network, see repository root for details.
+ *
+ *
+ * Some of the following code is derived from code original to the
+ * Iris project. That original code is
+ *
+ *	Copyright Iris developers and contributors
+ *
+ * and used according to the following license.
+ *
+ *	SPDX-License-Identifier: BSD-3-Clause
+ *
+ * Original Iris License:
+ * https://gitlab.mpi-sws.org/iris/iris/-/blob/d8ec293d24af02deb535e4cffc31a2de2fdf0344/LICENSE-CODE
+ *)
+
+From stdpp Require Import coPset namespaces.
+From iris.bi.lib Require Import fixpoint.
+From iris.proofmode Require Import coq_tactics tactics reduction.
+From iris.prelude Require Import options.
+From iris.bi.lib Require Import atomic.
+Require Import bedrock.bi.telescopes.
+Require Export bedrock.bi.lib.laterable.
+
+
+(** Conveniently split a conjunction on both assumption and conclusion. *)
+Local Tactic Notation "iSplitWith" constr(H) :=
+  iApply (bi.and_parallel with H); iSplit; iIntros H.
+
+Section definition.
+  Context `{BiFUpd PROP} {TA TB : tele}.
+  Implicit Types
+    (Eo Ei : coPset) (* outer/inner masks *)
+    (α : TA → PROP) (* atomic pre-condition *)
+    (P : PROP) (* abortion condition *)
+    (β : TA → TB → PROP) (* atomic post-condition *)
+    (Φ : TA → TB → PROP) (* post-condition *)
+  .
+
+  (** atomic1_acc as the "introduction form" of atomic updates: An accessor
+      that can be aborted back to [P]. *)
+  (* This one can make a step (having a later) for the COMMIT case. *)
+  Definition atomic1_acc Eo Ei α P β Φ : PROP :=
+    (|={Eo, Ei}=> ∃.. x, α x ∗
+          ((α x ={Ei, Eo}=∗ P) ∧ ▷ (∀.. y, β x y ={Ei, Eo}=∗ Φ x y))
+    )%I.
+
+  (* atomic1_acc is more restricted than atomic_acc *)
+  Lemma atomic_acc_atomic1_acc Eo Ei α P β Φ :
+    atomic_acc Eo Ei α P β Φ -∗ atomic1_acc Eo Ei α P β Φ.
+  Proof.
+    rewrite /atomic1_acc /atomic_acc.
+    iIntros "AS". iMod "AS" as (x) "[Hα Hclose]".
+    iModIntro. iExists x. iFrame "Hα". iSplit.
+    - iIntros "Hα". iDestruct "Hclose" as "[Hclose _]".
+      iApply "Hclose". done.
+    - iIntros "!>" (y) "Hβ". iDestruct "Hclose" as "[_ Hclose]".
+      iApply "Hclose". done.
+  Qed.
+
+  Lemma atomic1_acc_wand Eo Ei α P1 P2 β Φ1 Φ2 :
+    ((P1 -∗ P2) ∧ ▷ (∀.. x y, Φ1 x y -∗ Φ2 x y)) -∗
+    (atomic1_acc Eo Ei α P1 β Φ1 -∗ atomic1_acc Eo Ei α P2 β Φ2).
+  Proof.
+    iIntros "HP12 AS". iMod "AS" as (x) "[Hα Hclose]".
+    iModIntro. iExists x. iFrame "Hα". iSplit.
+    - iIntros "Hα". iDestruct "Hclose" as "[Hclose _]".
+      iApply "HP12". iApply "Hclose". done.
+    - iIntros "!>" (y) "Hβ". iDestruct "Hclose" as "[_ Hclose]".
+      iApply "HP12". iApply "Hclose". done.
+  Qed.
+
+  Lemma atomic1_acc_mask Eo Ed α P β Φ :
+    atomic1_acc Eo (Eo∖Ed) α P β Φ ⊣⊢ ∀ E, ⌜Eo ⊆ E⌝ → atomic1_acc E (E∖Ed) α P β Φ.
+  Proof.
+    iSplit; last first.
+    { iIntros "Hstep". iApply ("Hstep" with "[% //]"). }
+    iIntros "Hstep" (E HE).
+    iApply (fupd_mask_frame_acc with "Hstep"); first done.
+    iIntros "Hstep". iDestruct "Hstep" as (x) "[Hα Hclose]".
+    iIntros "!> Hclose'".
+    iExists x. iFrame. iSplitWith "Hclose".
+    - iIntros "Hα". iApply "Hclose'". iApply "Hclose". done.
+    - iIntros "!>" (y) "Hβ". iApply "Hclose'". iApply "Hclose". done.
+  Qed.
+
+  Lemma atomic1_acc_mask_weaken Eo1 Eo2 Ei α P β Φ :
+    Eo1 ⊆ Eo2 →
+    atomic1_acc Eo1 Ei α P β Φ -∗ atomic1_acc Eo2 Ei α P β Φ.
+  Proof.
+    iIntros (HE) "Hstep".
+    iMod fupd_intro_mask' as "Hclose1"; first done.
+    iMod "Hstep" as (x) "[Hα Hclose2]". iIntros "!>". iExists x.
+    iFrame. iSplitWith "Hclose2".
+    - iIntros "Hα". iMod ("Hclose2" with "Hα") as "$". done.
+    - iIntros "!>" (y) "Hβ". iMod ("Hclose2" with "Hβ") as "$". done.
+  Qed.
+
+  (** atomic1_update as a fixed-point of the equation
+   AU = make_laterable $ atomic1_acc α AU β Q
+  *)
+  Context Eo Ei α β Φ.
+
+  Definition atomic1_update_pre (Ψ : () → PROP) (_ : ()) : PROP :=
+    make_laterable $ atomic1_acc Eo Ei α (Ψ ()) β Φ.
+
+  Local Instance atomic1_update_pre_mono : BiMonoPred atomic1_update_pre.
+  Proof.
+    constructor.
+    - iIntros (P1 P2) "#HP12". iIntros ([]) "AU".
+      iApply (make_laterable_wand with "[] AU").
+      iIntros "!> AA". iApply (atomic1_acc_wand with "[HP12] AA").
+      iSplit; last by eauto. iApply "HP12".
+    - intros ??. solve_proper.
+  Qed.
+
+  Definition atomic1_update_def :=
+    bi_greatest_fixpoint atomic1_update_pre ().
+
+End definition.
+
+(** Seal it *)
+Definition atomic1_update_aux : seal (@atomic1_update_def). Proof. by eexists. Qed.
+Definition atomic1_update := atomic1_update_aux.(unseal).
+Global Arguments atomic1_update {PROP _ TA TB}.
+Definition atomic1_update_eq : @atomic1_update = _ := atomic1_update_aux.(seal_eq).
+
+Global Arguments atomic1_acc {PROP _ TA TB} Eo Ei _ _ _ _ : simpl never.
+Global Arguments atomic1_update {PROP _ TA TB} Eo Ei _ _ _ : simpl never.
+
+(** Notation: Atomic updates *)
+Notation "'AU1' '<<' ∀ x1 .. xn , α '>>' @ Eo , Ei '<<' ∃ y1 .. yn , β , 'COMM' Φ '>>'" :=
+  (atomic1_update (TA:=TeleS (λ x1, .. (TeleS (λ xn, TeleO)) .. ))
+                 (TB:=TeleS (λ y1, .. (TeleS (λ yn, TeleO)) .. ))
+                 Eo Ei
+                 (tele_app (TT:=TeleS (λ x1, .. (TeleS (λ xn, TeleO)) .. )) $
+                       λ x1, .. (λ xn, α%I) ..)
+                 (tele_app (TT:=TeleS (λ x1, .. (TeleS (λ xn, TeleO)) .. )) $
+                       λ x1, .. (λ xn,
+                         tele_app (TT:=TeleS (λ y1, .. (TeleS (λ yn, TeleO)) .. ))
+                         (λ y1, .. (λ yn, β%I) .. )
+                        ) .. )
+                 (tele_app (TT:=TeleS (λ x1, .. (TeleS (λ xn, TeleO)) .. )) $
+                       λ x1, .. (λ xn,
+                         tele_app (TT:=TeleS (λ y1, .. (TeleS (λ yn, TeleO)) .. ))
+                         (λ y1, .. (λ yn, Φ%I) .. )
+                        ) .. )
+  )
+  (at level 20, Eo, Ei, α, β, Φ at level 200, x1 binder, xn binder, y1 binder, yn binder,
+   format "'[   ' 'AU1'  '<<'  ∀  x1  ..  xn ,  α  '>>'  '/' @  Eo ,  Ei  '/' '[   ' '<<'  ∃  y1  ..  yn ,  β ,  '/' COMM  Φ  '>>' ']' ']'") : bi_scope.
+
+Notation "'AU1' '<<' ∀ x1 .. xn , α '>>' @ Eo , Ei '<<' β , 'COMM' Φ '>>'" :=
+  (atomic1_update (TA:=TeleS (λ x1, .. (TeleS (λ xn, TeleO)) .. ))
+                 (TB:=TeleO)
+                 Eo Ei
+                 (tele_app (TT:=TeleS (λ x1, .. (TeleS (λ xn, TeleO)) .. )) $
+                       λ x1, .. (λ xn, α%I) ..)
+                 (tele_app (TT:=TeleS (λ x1, .. (TeleS (λ xn, TeleO)) .. )) $
+                       λ x1, .. (λ xn, tele_app (TT:=TeleO) β%I) .. )
+                 (tele_app (TT:=TeleS (λ x1, .. (TeleS (λ xn, TeleO)) .. )) $
+                       λ x1, .. (λ xn, tele_app (TT:=TeleO) Φ%I) .. )
+  )
+  (at level 20, Eo, Ei, α, β, Φ at level 200, x1 binder, xn binder,
+   format "'[   ' 'AU1'  '<<'  ∀  x1  ..  xn ,  α  '>>'  '/' @  Eo ,  Ei  '/' '[   ' '<<'  β ,  '/' COMM  Φ  '>>' ']' ']'") : bi_scope.
+
+Notation "'AU1' '<<' α '>>' @ Eo , Ei '<<' ∃ y1 .. yn , β , 'COMM' Φ '>>'" :=
+  (atomic1_update (TA:=TeleO)
+                 (TB:=TeleS (λ y1, .. (TeleS (λ yn, TeleO)) .. ))
+                 Eo Ei
+                 (tele_app (TT:=TeleO) α%I)
+                 (tele_app (TT:=TeleO) $
+                       tele_app (TT:=TeleS (λ y1, .. (TeleS (λ yn, TeleO)) .. ))
+                                (λ y1, .. (λ yn, β%I) ..))
+                 (tele_app (TT:=TeleO) $
+                       tele_app (TT:=TeleS (λ y1, .. (TeleS (λ yn, TeleO)) .. ))
+                                (λ y1, .. (λ yn, Φ%I) ..))
+  )
+  (at level 20, Eo, Ei, α, β, Φ at level 200, y1 binder, yn binder,
+   format "'[   ' 'AU1'  '<<'  α  '>>'  '/' @  Eo ,  Ei  '/' '[   ' '<<'  ∃  y1  ..  yn ,  β ,  '/' COMM  Φ  '>>' ']' ']'") : bi_scope.
+
+Notation "'AU1' '<<' α '>>' @ Eo , Ei '<<' β , 'COMM' Φ '>>'" :=
+  (atomic1_update (TA:=TeleO) (TB:=TeleO) Eo Ei
+                 (tele_app (TT:=TeleO) α%I)
+                 (tele_app (TT:=TeleO) $ tele_app (TT:=TeleO) β%I)
+                 (tele_app (TT:=TeleO) $ tele_app (TT:=TeleO) Φ%I)
+  )
+  (at level 20, Eo, Ei, α, β, Φ at level 200,
+   format "'[   ' 'AU1'  '<<'  α  '>>'  '/' @  Eo ,  Ei  '/' '[   ' '<<'  β ,  '/' COMM  Φ  '>>' ']' ']'") : bi_scope.
+
+(** Notation: Atomic accessors *)
+Notation "'AACC1' '<<' ∀ x1 .. xn , α 'ABORT' P '>>' @ Eo , Ei '<<' ∃ y1 .. yn , β , 'COMM' Φ '>>'" :=
+  (atomic1_acc (TA:=TeleS (λ x1, .. (TeleS (λ xn, TeleO)) .. ))
+              (TB:=TeleS (λ y1, .. (TeleS (λ yn, TeleO)) .. ))
+              Eo Ei
+              (tele_app (TT:=TeleS (λ x1, .. (TeleS (λ xn, TeleO)) .. )) $
+                    λ x1, .. (λ xn, α%I) ..)
+              P%I
+              (tele_app (TT:=TeleS (λ x1, .. (TeleS (λ xn, TeleO)) .. )) $
+                    λ x1, .. (λ xn,
+                      tele_app (TT:=TeleS (λ y1, .. (TeleS (λ yn, TeleO)) .. ))
+                      (λ y1, .. (λ yn, β%I) .. )
+                     ) .. )
+              (tele_app (TT:=TeleS (λ x1, .. (TeleS (λ xn, TeleO)) .. )) $
+                    λ x1, .. (λ xn,
+                      tele_app (TT:=TeleS (λ y1, .. (TeleS (λ yn, TeleO)) .. ))
+                      (λ y1, .. (λ yn, Φ%I) .. )
+                     ) .. )
+  )
+  (at level 20, Eo, Ei, α, P, β, Φ at level 200, x1 binder, xn binder, y1 binder, yn binder,
+   format "'[     ' 'AACC1'  '[   ' '<<'  ∀  x1  ..  xn ,  α  '/' ABORT  P  '>>'  ']' '/' @  Eo ,  Ei  '/' '[   ' '<<'  ∃  y1  ..  yn ,  β ,  '/' COMM  Φ  '>>' ']' ']'") : bi_scope.
+
+Notation "'AACC1' '<<' ∀ x1 .. xn , α 'ABORT' P '>>' @ Eo , Ei '<<' β , 'COMM' Φ '>>'" :=
+  (atomic1_acc (TA:=TeleS (λ x1, .. (TeleS (λ xn, TeleO)) .. ))
+              (TB:=TeleO)
+              Eo Ei
+              (tele_app (TT:=TeleS (λ x1, .. (TeleS (λ xn, TeleO)) .. )) $
+                        λ x1, .. (λ xn, α%I) ..)
+              P%I
+              (tele_app (TT:=TeleS (λ x1, .. (TeleS (λ xn, TeleO)) .. )) $
+                        λ x1, .. (λ xn, tele_app (TT:=TeleO) β%I) .. )
+              (tele_app (TT:=TeleS (λ x1, .. (TeleS (λ xn, TeleO)) .. )) $
+                        λ x1, .. (λ xn, tele_app (TT:=TeleO) Φ%I) .. )
+  )
+  (at level 20, Eo, Ei, α, P, β, Φ at level 200, x1 binder, xn binder,
+   format "'[     ' 'AACC1'  '[   ' '<<'  ∀  x1  ..  xn ,  α  '/' ABORT  P  '>>'  ']' '/' @  Eo ,  Ei  '/' '[   ' '<<'  β ,  '/' COMM  Φ  '>>' ']' ']'") : bi_scope.
+
+Notation "'AACC1' '<<' α 'ABORT' P '>>' @ Eo , Ei '<<' ∃ y1 .. yn , β , 'COMM' Φ '>>'" :=
+  (atomic1_acc (TA:=TeleO)
+              (TB:=TeleS (λ y1, .. (TeleS (λ yn, TeleO)) .. ))
+              Eo Ei
+              (tele_app (TT:=TeleO) α%I)
+              P%I
+              (tele_app (TT:=TeleO) $
+                        tele_app (TT:=TeleS (λ y1, .. (TeleS (λ yn, TeleO)) .. ))
+                        (λ y1, .. (λ yn, β%I) ..))
+              (tele_app (TT:=TeleO) $
+                        tele_app (TT:=TeleS (λ y1, .. (TeleS (λ yn, TeleO)) .. ))
+                        (λ y1, .. (λ yn, Φ%I) ..))
+  )
+  (at level 20, Eo, Ei, α, P, β, Φ at level 200, y1 binder, yn binder,
+   format "'[     ' 'AACC1'  '[   ' '<<'  α  '/' ABORT  P  '>>'  ']' '/' @  Eo ,  Ei  '/' '[   ' '<<'  ∃  y1  ..  yn ,  β ,  '/' COMM  Φ  '>>' ']' ']'") : bi_scope.
+
+Notation "'AACC1' '<<' α 'ABORT' P '>>' @ Eo , Ei '<<' β , 'COMM' Φ '>>'" :=
+  (atomic1_acc (TA:=TeleO)
+              (TB:=TeleO)
+              Eo Ei
+              (tele_app (TT:=TeleO) α%I)
+              P%I
+                 (tele_app (TT:=TeleO) $ tele_app (TT:=TeleO) β%I)
+                 (tele_app (TT:=TeleO) $ tele_app (TT:=TeleO) Φ%I)
+  )
+  (at level 20, Eo, Ei, α, P, β, Φ at level 200,
+   format "'[     ' 'AACC1'  '[   ' '<<'  α  '/' ABORT  P  '>>'  ']' '/' @  Eo ,  Ei  '/' '[   ' '<<'  β ,  '/' COMM  Φ  '>>' ']' ']'") : bi_scope.
+
+(** Lemmas about AU *)
+Section lemmas.
+  Context `{BiFUpd PROP} {TA TB : tele}.
+  Implicit Types (α : TA → PROP) (β Φ : TA → TB → PROP) (P : PROP).
+
+  Local Existing Instances atomic1_update_pre_mono atomic_update_pre_mono.
+
+  (* Can't be in the section above as that fixes the parameters *)
+  Global Instance atomic1_acc_ne Eo Ei n :
+    Proper (
+        pointwise_relation TA (dist n) ==>
+        dist n ==>
+        pointwise_relation TA (pointwise_relation TB (dist n)) ==>
+        pointwise_relation TA (pointwise_relation TB (dist n)) ==>
+        dist n
+    ) (atomic1_acc (PROP:=PROP) Eo Ei).
+  Proof. solve_proper. Qed.
+
+  Global Instance atomic1_update_ne Eo Ei n :
+    Proper (
+        pointwise_relation TA (dist n) ==>
+        pointwise_relation TA (pointwise_relation TB (dist n)) ==>
+        pointwise_relation TA (pointwise_relation TB (dist n)) ==>
+        dist n
+    ) (atomic1_update (PROP:=PROP) Eo Ei).
+  Proof.
+    rewrite atomic1_update_eq /atomic1_update_def /atomic1_update_pre. solve_proper.
+  Qed.
+
+  (* AU implies AU1 *)
+  Lemma atomic_update_atomic1_update Eo Ei α β Φ :
+    atomic_update Eo Ei α β Φ -∗ atomic1_update Eo Ei α β Φ.
+  Proof.
+    rewrite atomic_update_eq atomic1_update_eq /atomic1_update_def /=.
+    iIntros "HAU".
+    iApply (greatest_fixpoint_coind _ (λ _, atomic_update_def Eo Ei α β Φ)); last done.
+    iIntros "!> *". rewrite {1}/atomic_update_def /= greatest_fixpoint_unfold.
+    iApply make_laterable_wand. iIntros "!>".
+    by iApply atomic_acc_atomic1_acc.
+  Qed.
+
+  Lemma atomic1_update_mask_weaken Eo1 Eo2 Ei α β Φ :
+    Eo1 ⊆ Eo2 →
+    atomic1_update Eo1 Ei α β Φ -∗ atomic1_update Eo2 Ei α β Φ.
+  Proof.
+    rewrite atomic1_update_eq {2}/atomic1_update_def /=.
+    iIntros (Heo) "HAU".
+    iApply (greatest_fixpoint_coind _ (λ _, atomic1_update_def Eo1 Ei α β Φ)); last done.
+    iIntros "!> *". rewrite {1}/atomic1_update_def /= greatest_fixpoint_unfold.
+    iApply make_laterable_wand. iIntros "!>".
+    iApply atomic1_acc_mask_weaken. done.
+  Qed.
+
+  (** The ellimination form: an atomic accessor *)
+  Lemma aupd1_aacc  Eo Ei α β Φ :
+    atomic1_update Eo Ei α β Φ -∗
+    atomic1_acc Eo Ei α (atomic1_update Eo Ei α β Φ) β Φ.
+  Proof using Type*.
+    rewrite atomic1_update_eq {1}/atomic1_update_def /=. iIntros "HUpd".
+    iPoseProof (greatest_fixpoint_unfold_1 with "HUpd") as "HUpd".
+    iApply make_laterable_elim. done.
+  Qed.
+
+  (* This lets you eliminate atomic updates with iMod. *)
+  Global Instance elim_mod_aupd1 φ Eo Ei E α β Φ Q Q' :
+    (∀ R, ElimModal φ false false (|={E,Ei}=> R) R Q Q') →
+    ElimModal (φ ∧ Eo ⊆ E) false false
+              (atomic1_update Eo Ei α β Φ)
+              (∃.. x, α x ∗
+                       (α x ={Ei,E}=∗ atomic1_update Eo Ei α β Φ) ∧
+                       ▷ (∀.. y, β x y ={Ei,E}=∗ Φ x y))
+              Q Q'.
+  Proof.
+    intros ?. rewrite /ElimModal /= =>-[??]. iIntros "[AU Hcont]".
+    iPoseProof (aupd1_aacc with "AU") as "AC".
+    iMod (atomic1_acc_mask_weaken with "AC"); first done.
+    iApply "Hcont". done.
+  Qed.
+
+  Global Instance aupd1_laterable Eo Ei α β Φ :
+    Laterable (atomic1_update Eo Ei α β Φ).
+  Proof.
+    rewrite atomic1_update_eq {1}/atomic1_update_def greatest_fixpoint_unfold.
+    apply _.
+  Qed.
+
+  Lemma aupd1_intro P Q α β Eo Ei Φ :
+    Affine P → Persistent P → Laterable Q →
+    (P ∗ Q -∗ atomic1_acc Eo Ei α Q β Φ) →
+    P ∗ Q -∗ atomic1_update Eo Ei α β Φ.
+  Proof.
+    rewrite atomic1_update_eq {1}/atomic1_update_def /=.
+    iIntros (??? HAU) "[#HP HQ]".
+    iApply (greatest_fixpoint_coind _ (λ _, Q)); last done. iIntros "!>" ([]) "HQ".
+    iApply (make_laterable_intro Q with "[] HQ"). iIntros "!> >HQ".
+    iApply HAU. by iFrame.
+  Qed.
+
+  Lemma aacc1_intro Eo Ei α P β Φ :
+    Ei ⊆ Eo → ⊢ (∀.. x, α x -∗
+    ((α x ={Eo}=∗ P) ∧ ▷ (∀.. y, β x y ={Eo}=∗ Φ x y)) -∗
+    atomic1_acc Eo Ei α P β Φ).
+  Proof.
+    iIntros (? x) "Hα Hclose".
+    iMod fupd_intro_mask' as "Hclose'"; last iModIntro; first set_solver.
+    iExists x. iFrame. iSplitWith "Hclose".
+    - iIntros "Hα". iMod "Hclose'" as "_". iApply "Hclose". done.
+    - iIntros "!>" (y) "Hβ". iMod "Hclose'" as "_". iApply "Hclose". done.
+  Qed.
+
+  (* This lets you open invariants etc. when the goal is an atomic accessor. *)
+  Global Instance elim_acc_aacc1 {X} E1 E2 Ei (α' β' : X → PROP) γ' α β Pas Φ :
+    ElimAcc (X:=X) True (fupd E1 E2) (fupd E2 E1) α' β' γ'
+            (atomic1_acc E1 Ei α Pas β Φ)
+            (λ x', atomic1_acc E2 Ei α (β' x' ∗ (γ' x' -∗? Pas))%I β
+                (λ.. x y, β' x' ∗ (γ' x' -∗? Φ x y))
+            )%I.
+  Proof.
+    (* FIXME: Is there any way to prevent maybe_wand from unfolding?
+       It gets unfolded by env_cbv in the proofmode, ideally we'd like that
+       to happen only if one argument is a constructor. *)
+    iIntros (_) "Hinner >Hacc". iDestruct "Hacc" as (x') "[Hα' Hclose]".
+    iMod ("Hinner" with "Hα'") as (x) "[Hα Hclose']".
+    iMod (fupd_intro_mask') as "Hclose''"; last iModIntro; first done.
+    iExists x. iFrame. iSplitWith "Hclose'".
+    - iIntros "Hα". iMod "Hclose''" as "_".
+      iMod ("Hclose'" with "Hα") as "[Hβ' HPas]".
+      iMod ("Hclose" with "Hβ'") as "Hγ'".
+      iModIntro. destruct (γ' x'); iApply "HPas"; done.
+    - iIntros "!>" (y) "Hβ". iMod "Hclose''" as "_".
+      iMod ("Hclose'" with "Hβ") as "Hβ'".
+      (* FIXME: Using ssreflect rewrite does not work, see Coq bug #7773. *)
+      rewrite ->!tele_app_bind. iDestruct "Hβ'" as "[Hβ' HΦ]".
+      iMod ("Hclose" with "Hβ'") as "Hγ'".
+      iModIntro. destruct (γ' x'); iApply "HΦ"; done.
+  Qed.
+
+  (* Everything that fancy updates can eliminate without changing, atomic
+  accessors can eliminate as well.  This is a forwarding instance needed becuase
+  atomic1_acc is becoming opaque. *)
+  Global Instance elim_modal_acc p q φ P P' Eo Ei α Pas β Φ :
+    (∀ Q, ElimModal φ p q P P' (|={Eo,Ei}=> Q) (|={Eo,Ei}=> Q)) →
+    ElimModal φ p q P P'
+              (atomic1_acc Eo Ei α Pas β Φ)
+              (atomic1_acc Eo Ei α Pas β Φ).
+  Proof. intros Helim. apply Helim. Qed.
+
+  Lemma aacc1_aacc {TA' TB' : tele} E1 E1' E2 E3
+        α P β Φ
+        (α' : TA' → PROP) P' (β' Φ' : TA' → TB' → PROP) :
+    E1' ⊆ E1 →
+    atomic1_acc E1' E2 α P β Φ -∗
+    (∀.. x, α x -∗ atomic1_acc E2 E3 α' (α x ∗ (P ={E1}=∗ P')) β'
+            (λ.. x' y', (α x ∗ (P ={E1}=∗ Φ' x' y'))
+                    ∨ ∃.. y, β x y ∗ (Φ x y ={E1}=∗ Φ' x' y'))) -∗
+    atomic1_acc E1 E3 α' P' β' Φ'.
+  Proof.
+    iIntros (?) "Hupd Hstep".
+    iMod (atomic1_acc_mask_weaken with "Hupd") as (x) "[Hα Hclose]"; first done.
+    iMod ("Hstep" with "Hα") as (x') "[Hα' Hclose']".
+    iModIntro. iExists x'. iFrame "Hα'". iSplit.
+    - iIntros "Hα'". iDestruct "Hclose'" as "[Hclose' _]".
+      iMod ("Hclose'" with "Hα'") as "[Hα Hupd]".
+      iDestruct "Hclose" as "[Hclose _]".
+      iMod ("Hclose" with "Hα"). iApply "Hupd". auto.
+    - iIntros "!>" (y') "Hβ'". iDestruct "Hclose'" as "[_ Hclose']".
+      iMod ("Hclose'" with "Hβ'") as "Hres".
+      (* FIXME: Using ssreflect rewrite does not work, see Coq bug #7773. *)
+      rewrite ->!tele_app_bind. iDestruct "Hres" as "[[Hα HΦ']|Hcont]".
+      + (* Abort the step we are eliminating *)
+        iDestruct "Hclose" as "[Hclose _]".
+        iMod ("Hclose" with "Hα") as "HP".
+        iApply "HΦ'". done.
+      + (* Complete the step we are eliminating *)
+        iDestruct "Hclose" as "[_ Hclose]".
+        iDestruct "Hcont" as (y) "[Hβ HΦ']".
+        iMod ("Hclose" with "Hβ") as "HΦ".
+        iApply "HΦ'". done.
+  Qed.
+
+  Lemma aacc1_aupd {TA' TB' : tele} E1 E1' E2 E3
+        α β Φ
+        (α' : TA' → PROP) P' (β' Φ' : TA' → TB' → PROP) :
+    E1' ⊆ E1 →
+    atomic1_update E1' E2 α β Φ -∗
+    (∀.. x, α x -∗ atomic1_acc E2 E3 α' (α x ∗ (atomic1_update E1' E2 α β Φ ={E1}=∗ P')) β'
+            (λ.. x' y', (α x ∗ (atomic1_update E1' E2 α β Φ ={E1}=∗ Φ' x' y'))
+                    ∨ ∃.. y, β x y ∗ (Φ x y ={E1}=∗ Φ' x' y'))) -∗
+    atomic1_acc E1 E3 α' P' β' Φ'.
+  Proof.
+    iIntros (?) "Hupd Hstep". iApply (aacc1_aacc with "[Hupd] Hstep"); first done.
+    iApply aupd1_aacc; done.
+  Qed.
+
+  Lemma aacc1_aupd_commit {TA' TB' : tele} E1 E1' E2 E3
+        α β Φ
+        (α' : TA' → PROP) P' (β' Φ' : TA' → TB' → PROP) :
+    E1' ⊆ E1 →
+    atomic1_update E1' E2 α β Φ -∗
+    (∀.. x, α x -∗ atomic1_acc E2 E3 α' (α x ∗ (atomic1_update E1' E2 α β Φ ={E1}=∗ P')) β'
+            (λ.. x' y', ∃.. y, β x y ∗ (Φ x y ={E1}=∗ Φ' x' y'))) -∗
+    atomic1_acc E1 E3 α' P' β' Φ'.
+  Proof.
+    iIntros (?) "Hupd Hstep". iApply (aacc1_aupd with "Hupd"); first done.
+    iIntros (x) "Hα". iApply atomic1_acc_wand; last first.
+    { iApply "Hstep". done. }
+    (* FIXME: Using ssreflect rewrite does not work, see Coq bug #7773. *)
+    iSplit; first by eauto. iIntros "!>" (??) "?". rewrite ->!tele_app_bind. by iRight.
+  Qed.
+
+  Lemma aacc1_aupd_abort {TA' TB' : tele} E1 E1' E2 E3
+        α β Φ
+        (α' : TA' → PROP) P' (β' Φ' : TA' → TB' → PROP) :
+    E1' ⊆ E1 →
+    atomic1_update E1' E2 α β Φ -∗
+    (∀.. x, α x -∗ atomic1_acc E2 E3 α' (α x ∗ (atomic1_update E1' E2 α β Φ ={E1}=∗ P')) β'
+            (λ.. x' y', α x ∗ (atomic1_update E1' E2 α β Φ ={E1}=∗ Φ' x' y'))) -∗
+    atomic1_acc E1 E3 α' P' β' Φ'.
+  Proof.
+    iIntros (?) "Hupd Hstep". iApply (aacc1_aupd with "Hupd"); first done.
+    iIntros (x) "Hα". iApply atomic1_acc_wand; last first.
+    { iApply "Hstep". done. }
+    (* FIXME: Using ssreflect rewrite does not work, see Coq bug #7773. *)
+    iSplit; first by eauto. iIntros "!>" (??) "?". rewrite ->!tele_app_bind. by iLeft.
+  Qed.
+
+End lemmas.
+
+
+Section atomic.
+  Context `{BiFUpd PROP} {TA TB : tele}.
+  Implicit Types (α : TA → PROP).
+  Implicit Types (β Φ : TA → TB → PROP).
+
+  Global Instance aacc1_proper Eo Ei :
+    Proper (
+      pointwise_relation TA (≡) ==>
+      (≡) ==>
+      pointwise_relation TA (pointwise_relation TB (≡)) ==>
+      pointwise_relation TA (pointwise_relation TB (≡)) ==>
+      (≡)
+    ) (atomic1_acc (PROP:=PROP) Eo Ei).
+  Proof. solve_proper. Qed.
+
+  Global Instance aacc1_mono' Eo Ei :
+    Proper (
+      pointwise_relation TA (≡) ==>
+      (⊢) ==>
+      pointwise_relation TA (pointwise_relation TB (flip (⊢))) ==>
+      pointwise_relation TA (pointwise_relation TB (⊢)) ==>
+      (⊢)
+    ) (atomic1_acc (PROP:=PROP) Eo Ei).
+  Proof.
+    intros α1 α2 Hα P1 P2 HP β1 β2 Hβ Φ1 Φ2 HΦ. rewrite/atomic1_acc.
+    repeat f_equiv; by rewrite ?Hα ?HP.
+  Qed.
+
+  Global Instance aacc1_flip_mono' Eo Ei :
+    Proper (
+      pointwise_relation TA (≡) ==>
+      flip (⊢) ==>
+      pointwise_relation TA (pointwise_relation TB (⊢)) ==>
+      pointwise_relation TA (pointwise_relation TB (flip (⊢))) ==>
+      flip (⊢)
+    ) (atomic1_acc (PROP:=PROP) Eo Ei).
+  Proof. repeat intro. by rewrite -aacc1_mono'. Qed.
+
+  Global Instance aupd1_proper Eo Ei :
+    Proper (
+      pointwise_relation TA (≡) ==>
+      pointwise_relation TA (pointwise_relation TB (≡)) ==>
+      pointwise_relation TA (pointwise_relation TB (≡)) ==>
+      (≡)
+    ) (atomic1_update (PROP:=PROP) Eo Ei).
+  Proof.
+    rewrite atomic1_update_eq /atomic1_update_def /atomic1_update_pre.
+    solve_proper.
+  Qed.
+
+  Global Instance aupd1_mono' Eo Ei :
+    Proper (
+      pointwise_relation TA (≡) ==>
+      pointwise_relation TA (pointwise_relation TB (flip (⊢))) ==>
+      pointwise_relation TA (pointwise_relation TB (⊢)) ==>
+      (⊢)
+    ) (atomic1_update (PROP:=PROP) Eo Ei).
+  Proof.
+    rewrite atomic1_update_eq /atomic1_update_def /atomic1_update_pre.
+    solve_proper.
+  Qed.
+
+  Global Instance aupd1_flip_mono' Eo Ei :
+    Proper (
+      pointwise_relation TA (≡) ==>
+      pointwise_relation TA (pointwise_relation TB (⊢)) ==>
+      pointwise_relation TA (pointwise_relation TB (flip (⊢))) ==>
+      flip (⊢)
+    ) (atomic1_update (PROP:=PROP) Eo Ei).
+  Proof. repeat intro. by rewrite -aupd1_mono'. Qed.
+
+End atomic.
+
+(** The tactic [iAuIntro] applies lemma [aupd_aacc] to change an Iris
+proof mode goal [P := atomic_update Eo Ei α β Φ] into [atomic_acc Eo
+Ei α P β Φ] _provided_ everything in the proof mode's spatial context
+is [Laterable] (e.g., [Timeless], an atomic update, or something under
+the later modality).
+
+Our version of the tactic generalizes the Iris original to avoid its
+[Timeless emp] assumption when the spatial context is non-empty. *)
+
+Section coq_tactic.
+  Import coq_tactics.
+  Context `{BiFUpd PROP} {TA TB : tele}.
+  Implicit Types (α : TA → PROP).
+  Implicit Types (β Φ : TA → TB → PROP).
+
+  Lemma tac_aupd1_intro Γp Γs n α β Eo Ei Φ P :
+    TCOr (ListNonEmpty (env_to_list Γs)) (Timeless (PROP:=PROP) emp) →
+    TCForall Laterable (env_to_list Γs) →
+    P = env_to_prop Γs →
+    envs_entails (Envs Γp Γs n) (atomic1_acc Eo Ei α P β Φ) →
+    envs_entails (Envs Γp Γs n) (atomic1_update Eo Ei α β Φ).
+  Proof.
+    intros ?? ->. rewrite envs_entails_eq of_envs_eq' /=.
+    rewrite env_to_prop_sound=>?. exact: aupd1_intro.
+  Qed.
+End coq_tactic.
+
+Lemma test_before `{BiFUpd PROP} {TA TB : tele} Eo Ei α (β Φ : TA → TB → PROP) :
+  atomic1_update Eo Ei α β Φ ⊢ atomic1_update Eo Ei α β Φ.
+Proof. iIntros "AU". Fail iAuIntro. Abort.
+
+Tactic Notation "iAuIntro1" :=
+  iStartProof; eapply tac_aupd1_intro; [
+    iSolveTC || fail "iAuIntro1: emp is not timeless"
+  | iSolveTC || fail "iAuIntro1: not all spatial assumptions are laterable"
+  | (* P = ...: make the P pretty *) reduction.pm_reflexivity
+  | (* the new proof mode goal *) ].
+Lemma test_after `{BiFUpd PROP} {TA TB : tele} Eo Ei α (β Φ : TA → TB → PROP) :
+  atomic1_update Eo Ei α β Φ ⊢ atomic1_update Eo Ei α β Φ.
+Proof. iIntros "AU". iAuIntro1. Abort.
+
+Tactic Notation "iAaccIntro1" "with" constr(sel) :=
+  iStartProof; lazymatch goal with
+  | |- environments.envs_entails _ (@atomic1_acc ?PROP ?H ?TA ?TB ?Eo ?Ei ?α ?P ?β ?Φ) =>
+    iApply (@aacc1_intro PROP H TA TB Eo Ei α P β Φ with sel);
+    first try solve_ndisj; last iSplit
+  | _ => fail "iAaccIntro1: Goal is not an atomic accessor"
+  end.
+
+(* From here on, prevent TC search from implicitly unfolding these. *)
+Typeclasses Opaque atomic1_acc atomic1_update.
